Prove on pi steps

src/drf/PromiseIndep.v
@@ -17,20 +17,47 @@ Require Import Configuration.
 Set Implicit Arguments.
 
 
+Inductive small_step (e:ThreadEvent.t) (tid:Ident.t) (c1:Configuration.t): forall (c2:Configuration.t), Prop :=
+| small_step_intro
+    lang st1 lc1 st2 lc2 memory2
+    (TID: IdentMap.find tid c1.(Configuration.threads) = Some (existT _ lang st1, lc1))
+    (STEP: Thread.step e (Thread.mk _ st1 lc1 c1.(Configuration.memory)) (Thread.mk _ st2 lc2 memory2)):
+    small_step e tid c1 (Configuration.mk (IdentMap.add tid (existT _ _ st2, lc2) c1.(Configuration.threads)) memory2)
+.
+
+Inductive tau_small_step (tid:Ident.t) (c1 c2:Configuration.t): Prop :=
+| tau_small_step_intro
+    e
+    (STEP: small_step e tid c1 c2)
+    (TAU: ThreadEvent.get_event e = None)
+.
+
+Lemma step_small_steps
+      e tid c1 c3
+      (STEP: Configuration.step e tid c1 c3)
+      (CONSISTENT1: Configuration.consistent c1):
+  exists te c2,
+    <<STEPS: rtc (tau_small_step tid) c1 c2>> /\
+    <<STEP: small_step te tid c2 c3>> /\
+    <<EVENT: e = ThreadEvent.get_event te>> /\
+    <<CONSISTENT3: Configuration.consistent c3>>.
+Proof.
+  exploit Configuration.step_consistent; eauto. i. des.
+  admit.
+Admitted.
+
+
 Definition pi_machine_event (e:ThreadEvent.t) (threads:Threads.t): Prop :=
-  match e with
-  | ThreadEvent.read loc ts val ord => ~ Threads.is_promised loc ts threads
-  | ThreadEvent.update loc tsr tsw valr valw ordr ordw => ~ Threads.is_promised loc tsr threads
-  | _ => True
+  match ThreadEvent.is_reading e with
+  | Some (loc, ts, _) => ~ Threads.is_promised loc ts threads
+  | None => True
   end.
 
-Inductive pi_step (tid:Ident.t) (c1:Configuration.t): forall (c2:Configuration.t), Prop :=
+Inductive pi_step (tid:Ident.t) (c1 c2:Configuration.t): Prop :=
 | pi_step_intro
-    e lang st1 lc1 st2 lc2 memory2
-    (TID: IdentMap.find tid c1.(Configuration.threads) = Some (existT _ lang st1, lc1))
-    (STEP: Thread.step e (Thread.mk _ st1 lc1 c1.(Configuration.memory)) (Thread.mk _ st2 lc2 memory2))
-    (READINFO: pi_machine_event e c1.(Configuration.threads)):
-    pi_step tid c1 (Configuration.mk (IdentMap.add tid (existT _ _ st2, lc2) c1.(Configuration.threads)) memory2)
+    e
+    (STEP: small_step e tid c1 c2)
+    (READINFO: pi_machine_event e c1.(Configuration.threads))
 .
 
 Inductive pi_step_all (c1 c2:Configuration.t): Prop :=
@@ -61,7 +88,7 @@ Lemma pi_step_find
       (TID: tid1 <> tid2):
   IdentMap.find tid2 c2.(Configuration.threads) = IdentMap.find tid2 c1.(Configuration.threads).
 Proof.
-  inv STEP. s. rewrite IdentMap.Facts.add_neq_o; auto.
+  inv STEP. inv STEP0. s. rewrite IdentMap.Facts.add_neq_o; auto.
 Qed.
 
 Lemma rtc_pi_step_find
@@ -100,19 +127,70 @@ Definition pi_racefree (c1:Configuration.t): Prop :=
     <<ORDR: Ordering.le Ordering.acqrel ordr>> /\
     <<ORDW: Ordering.le Ordering.acqrel ordw>>.
 
-Lemma pi_consistent_step_pi_step
+Lemma pi_consistent_small_step_pi
+      e tid c1 c2 c3
+      (PI_CONSISTENT: pi_consistent c1)
+      (PI_RACEFREE: pi_racefree c1)
+      (PI_STEPS: rtc (pi_step tid) c1 c2)
+      (STEP: small_step e tid c2 c3):
+  pi_machine_event e c2.(Configuration.threads).
+Proof.
+  unfold pi_machine_event. destruct (ThreadEvent.is_reading e) as [[[]]|] eqn:E; auto. ii.
+  inv H.
+  assert (tid <> tid0).
+  { admit. }
+  exploit PI_CONSISTENT.
+  { erewrite <- rtc_pi_step_find; eauto. congr. }
+  { eapply rtc_implies; try apply PI_STEPS; eauto.
+    i. econs; eauto.
+  }
+  i. des. exploit PI_RACEFREE.
+  { etrans.
+    - eapply rtc_implies; try apply PI_STEPS; eauto.
+      i. econs; eauto.
+    - eapply rtc_implies; try apply STEPS; eauto.
+      i. econs; eauto.
+  }
+  { admit. (* race_rw *) }
+  { i. des. admit. (* rel -> contradiction *) }
+Admitted.
+
+Lemma pi_consistent_rtc_tau_small_step_pi
+      tid c1 c2 c3
+      (PI_CONSISTENT: pi_consistent c1)
+      (PI_RACEFREE: pi_racefree c1)
+      (PI_STEPS: rtc (pi_step tid) c1 c2)
+      (STEP: rtc (tau_small_step tid) c2 c3):
+  rtc (pi_step tid) c2 c3.
+Proof.
+  apply Operators_Properties.clos_rt_rt1n_iff in STEP.
+  apply Operators_Properties.clos_rt_rtn1_iff in STEP.
+  induction STEP; auto. etrans; eauto. econs 2; [|econs 1].
+  inv H. econs; eauto. eapply pi_consistent_small_step_pi; eauto.
+  etrans; eauto.
+Qed.
+
+Lemma pi_consistent_step_pi
       c1 c2
       e tid
       (PI_CONSISTENT: pi_consistent c1)
+      (CONSISTENT: Configuration.consistent c1)
+      (PI_RACEFREE: pi_racefree c1)
       (STEP: Configuration.step e tid c1 c2):
   rtc (pi_step tid) c1 c2.
 Proof.
-Admitted.
+  exploit step_small_steps; eauto. i. des. subst.
+  exploit pi_consistent_rtc_tau_small_step_pi; eauto. i.
+  exploit pi_consistent_small_step_pi; eauto. i.
+  etrans; eauto. econs 2; [|econs 1]. econs; eauto.
+Qed.
 
 Lemma pi_consistent_pi_step_pi_consistent
       c1 c2
       tid
       (PI_CONSISTENT: pi_consistent c1)
+      (CONSISTENT1: Configuration.consistent c1)
+      (CONSISTENT2: Configuration.consistent c2)
       (STEP: rtc (pi_step tid) c1 c2):
   pi_consistent c2.
 Proof.
