src/opt/Merge.v
@@ -1,0 +1,54 @@
+Require Import Basics.
+Require Import Bool.
+Require Import List.
+
+Require Import sflib.
+Require Import paco.
+Require Import respectful5.
+
+Require Import Basic.
+Require Import Event.
+Require Import Language.
+Require Import Time.
+Require Import Memory.
+Require Import Commit.
+Require Import Thread.
+
+Require Import Configuration.
+Require Import Simulation.
+Require Import Compatibility.
+Require Import MemInv.
+Require Import MergeStep.
+
+Require Import Syntax.
+Require Import Semantics.
+
+Set Implicit Arguments.
+
+Lemma merge_load_load_sim_stmts
+      l
+      r1 o1
+      r2 o2
+      o
+      (O1: Ordering.le o1 o)
+      (O2: Ordering.le o2 o):
+  sim_stmts eq
+            [Stmt.instr (Instr.load r1 l o1); Stmt.instr (Instr.load r2 l o2); Stmt.instr Instr.skip]
+            [Stmt.instr (Instr.load r1 l o); Stmt.instr (Instr.assign r2 (Instr.expr_val (Value.reg r1)))]
+            eq.
+Proof.
+  pcofix CIH. ii. subst. pfold. ii. splits.
+  { i. inv TERMINAL_TGT. }
+  { i. eapply sim_local_future; try apply MEMORY; eauto. apply LOCAL. }
+  { i. eexists _, _, _. splits; eauto.
+    inv LOCAL. apply MemInv.sem_bot_inv in PROMISES. rewrite PROMISES. auto.
+  }
+  ii. inv STEP_TGT; inv STEP; try (inv STATE; inv INSTR); ss.
+  - (* promise *)
+    exploit sim_local_promise; eauto. i. des.
+    eexists _, _, _, _, _, _, _. splits; eauto.
+    econs 1; eauto. econs; eauto. eauto.
+  - (* load *)
+    exploit merge_read_read; try apply LOCAL0; eauto. i. des.
+    admit.
+Admitted.
