src/opt/MergeCommit.v
@@ -129,22 +129,9 @@ Proof.
   - etrans; eauto. etrans; [apply WF|]. etrans; apply WF.
 Qed.
 
-Lemma write_write
-      loc ord
-      ts1 ord1
-      ts2 released2 ord2
-      commit0 commit2
-      (ORD1: Ordering.le ord1 ord)
-      (ORD2: Ordering.le ord2 ord)
-      (RW1: Time.lt (commit0.(Commit.cur).(Capability.rw) loc) ts1)
-      (TS: Time.lt ts1 ts2)
-      (COMMIT: Commit.write commit0 loc ts2 released2 ord commit2)
-      (WF0: Commit.wf commit0):
-  exists released1,
-    <<COMMIT1': Commit.write commit0 loc ts1 released1 ord1 (CommitFacts.write_min loc ts1 released1 commit0)>> /\
-    <<COMMIT2': Commit.write (CommitFacts.write_min loc ts1 released1 commit0) loc ts2 released2 ord2 commit2>>.
-Proof.
-Admitted.
+
+(* TODO: WW merge *)
+
 
 Lemma read_fence_read_fence
       ord1 ord2 ord
